lambda wp nary+prim done

theories/LambdaWP.v
@@ -278,19 +278,26 @@ Definition wp_getval wp (E:ctx) (t1:trm) (F2of:val->formula) : formula :=
   | _ => wp_let (wp E t1) F2of
   end.
 
-Definition wp_app_val (v0:val) (vs:vals) : formula := 
-  match v0 with
-  | val_prim val_eq => wp_binop (fun v1 v2 => isTrue (v1 + v2))
-  | val_prim val_add => wp_binop_int (fun n1 n2 => n1 + n2)
-  (* TODO: other primitives *)
-  | _ => local (wp_triple (trm_apps v0 vs))
-  end.
+Definition wp_unop_int (v1:val) (F:int->val) : formula := local (fun Q =>
+  \exists n1, \[v1 = val_int n1] \* Q (F n1)).
 
-(* Definition wp_app_val (E:ctx) (t:trm) : formula := 
-  local (wp_triple (isubst E t)). *)
-  (* Note that the substitution is usually the identity
-     because [t] is the application of a value to values *)
-    (* wp_app_val E (trm_apps v0 (trms_vals (List.rev rvs))) *)
+Definition wp_unop_bool (v1:val) (F:bool->val) : formula := local (fun Q =>
+  \exists b1, \[v1 = val_bool b1] \* Q (F b1)).
+
+Definition wp_binop_int (v1 v2:val) (F:int->int->val) : formula := local (fun Q =>
+  \exists n1 n2, \[v1 = val_int n1 /\ v2 = val_int n2] \* Q (F n1 n2)).
+
+Definition wp_apps_val (v0:val) (vs:vals) : formula := 
+  match v0, vs with
+  | val_prim val_opp, (v1::nil) => wp_unop_int v1 (fun n1 => - n1)
+  | val_prim val_neg, (v1::nil) => wp_unop_bool v1 (fun b1 => neg b1)
+  | val_prim val_eq, (v1::v2::nil) => wp_val (isTrue (v1 = v2))
+  | val_prim val_neq, (v1::v2::nil) => wp_val (isTrue (v1 <> v2))
+  | val_prim val_add, (v1::v2::nil) => wp_binop_int v1 v2 (fun n1 n2 => n1 + n2)
+  | val_prim val_sub, (v1::v2::nil) => wp_binop_int v1 v2 (fun n1 n2 => n1 - n2)
+  | val_prim val_mul, (v1::v2::nil) => wp_binop_int v1 v2 (fun n1 n2 => n1 * n2)
+  | _, _ => local (wp_triple (trm_apps v0 vs))
+  end.  (* not included: arithmetic comparisons *)
 
 Definition wp_apps wp (E:ctx) (v0:val) : list val -> list trm -> formula := 
   (fix mk (rvs : list val) (ts : list trm) : formula :=
@@ -338,7 +345,11 @@ Fixpoint wp (E:ctx) (t:trm) : formula :=
   match t with
   | trm_val v => wp_val v
   | trm_var x => wp_var E x
-  | trm_fixs f xs t1 => wp_val (val_fixs f xs (isubst (Ctx.rem_vars xs (Ctx.rem f E)) t1))
+  | trm_fixs f xs t1 => 
+      match xs with 
+      | nil => wp_fail
+      | _ => wp_val (val_fixs f xs (isubst (Ctx.rem_vars xs (Ctx.rem f E)) t1))
+      end
   | trm_constr id ts => wp_constr wp E id nil ts
   | trm_if t0 t1 t2 => wp_if (aux t0) (aux t1) (aux t2)
   | trm_let x t1 t2 => wp_let (aux t1) (fun X => wp (Ctx.add x X E) t2)
@@ -372,6 +383,13 @@ Proof using. intros. applys is_local_weakestpre. applys is_local_triple. Qed.
 Lemma triple_eq_himpl_wp_triple : forall H Q t,
   triple t H Q = (H ==> wp_triple t Q).
 Proof using. intros. applys weakestpre_eq. applys is_local_triple. Qed.
+
+(** Reformulation of the right-to-left implication above as an implication. *)
+
+Lemma triple_of_wp : forall H Q t,
+  H ==> wp_triple t Q ->
+  triple t H Q.
+Proof using. intros. rewrite* triple_eq_himpl_wp_triple. Qed.
 
 (** Reformulation of the left-to-right implication above in the form
     of an entailment. *)
@@ -438,7 +456,7 @@ Proof using. intros. intros Q. applys himpl_wp_fail_l. Qed.
 Lemma triple_wp_fail : forall t Q Q',
   triple t (wp_fail Q) Q'.
 Proof using. 
-  intros. rewrite triple_eq_himpl_wp_triple. applys himpl_wp_fail_l.
+  intros. apply triple_of_wp. applys himpl_wp_fail_l.
 Qed.
 
 (** Soundness of the [wp] for the various constructs *)
@@ -454,17 +472,17 @@ Proof using.
   introv HC M1 M2. applys qimpl_wp_triple. simpl. intros Q.
   tests C1: (trm_is_val t1).
   { destruct C1 as (v&Et). subst. simpl. 
-    rewrite triple_eq_himpl_wp_triple. applys M2. }
+    apply triple_of_wp. applys M2. }
   tests C2: (trm_is_var t1).
   { destruct C2 as (x&Et). subst. simpl. case_eq (Ctx.lookup x E).
     { intros v Ev. rewrites~ (>> isubst_evalctx_trm_var Ev).
-      rewrite triple_eq_himpl_wp_triple. applys M2. }
+      apply triple_of_wp. applys M2. }
     { introv N. remove_local. intros; false. } }
   asserts_rewrite (wp_getval wp E t1 F2of = wp_let (wp E t1) F2of).
   { destruct t1; auto. { false C1. hnfs*. } { false C2. hnfs*. } }
   remove_local. applys~ triple_isubst_evalctx.
-  { rewrite triple_eq_himpl_wp_triple. applys M1. }
-  { intros v. rewrite triple_eq_himpl_wp_triple. applys M2. }
+  { apply triple_of_wp. applys M1. }
+  { intros v. apply triple_of_wp. applys M2. }
 Qed.
 
 Lemma wp_sound_fail :
@@ -487,11 +505,13 @@ Proof using.
   intros Q. remove_local. applys~ triple_val.
 Qed.
 
-Lemma wp_sound_fix : forall f x t,
-  wp_sound (trm_fix f x t).
+Lemma wp_sound_fixs : forall f xs t,
+  wp_sound (trm_fixs f xs t).
 Proof using.
-  intros. intros E. applys qimpl_wp_triple. simpl.
-  intros Q. remove_local. applys~ triple_fix.
+  intros. intros E. applys qimpl_wp_triple. simpl. intros Q.
+  destruct xs as [|x xs'].
+  { applys~ triple_wp_fail. }
+  { remove_local. applys~ triple_fixs. auto_false. }
 Qed.
 
 Lemma wp_sound_if : forall F1 F2 F3 E t1 t2 t3,
@@ -502,10 +522,10 @@ Lemma wp_sound_if : forall F1 F2 F3 E t1 t2 t3,
 Proof using.
   introv M1 M2 M3. applys qimpl_wp_triple. simpl. intros Q.
   remove_local. applys triple_if.
-  { rewrite triple_eq_himpl_wp_triple. applys* M1. }
+  { apply triple_of_wp. applys* M1. }
   { intros b. simpl. remove_local ;=> b' M. inverts M. case_if.
-    { rewrite triple_eq_himpl_wp_triple. applys* M2. }
-    { rewrite triple_eq_himpl_wp_triple. applys* M3. } }
+    { apply triple_of_wp. applys* M2. }
+    { apply triple_of_wp. applys* M3. } }
   { introv N. applys local_false. intros Q'.
     hpull ;=> v' ->. false* N. hnfs*. }
 Qed.
@@ -517,8 +537,8 @@ Lemma wp_sound_let : forall F1 F2 E x t1 t2,
 Proof using.
   introv M1 M2. applys qimpl_wp_triple. simpl. intros Q.
   remove_local. applys triple_let.
-  { rewrite triple_eq_himpl_wp_triple. applys* M1. }
-  { intros X. simpl. rewrite triple_eq_himpl_wp_triple.
+  { apply triple_of_wp. applys* M1. }
+  { intros X. simpl. apply triple_of_wp.
     rewrite <- isubst_add_eq_subst1_isubst. applys* M2. }
 Qed.
 
@@ -529,47 +549,85 @@ Lemma wp_sound_seq : forall F1 F2 E t1 t2,
 Proof using.
   introv M1 M2. applys qimpl_wp_triple. simpl. intros Q.
   remove_local. applys triple_seq.
-  { rewrite triple_eq_himpl_wp_triple. applys* M1. }
-  { intros X. simpl. rewrite triple_eq_himpl_wp_triple. applys* M2. }
+  { apply triple_of_wp. applys* M1. }
+  { intros X. simpl. apply triple_of_wp. applys* M2. }
 Qed.
 
-Lemma wp_sound_app_val : forall E t,
-  wp_app_val E t ===> wp_triple_ E t.
+Lemma wp_sound_redbinop : forall v op v1 v2,
+  redbinop op v1 v2 v ->
+  wp_val v ===> wp_triple (trm_apps op (trms_vals (v1::v2::nil))).
 Proof using.
-  intros. intros Q. unfold wp_app_val. applys~ local_erase_l.
-  applys is_local_wp_triple.
+  introv M. applys qimpl_wp_triple; intros Q; simpl.
+  remove_local. applys triple_combined.
+  { applys triple_binop M. } { hsimpl. } { hpull ;=> ? ->. hsimpl. }
 Qed.
 
-
-Axiom evalctx_app2 : forall t1,
-      evalctx (fun t2 => trm_app t1 t2).
-Axiom evalctx_app1 : forall t2,
-      evalctx (fun t1 => trm_app t1 t2) .
-
-Lemma wp_sound_app : forall E t,
-  (forall ti, wp_sound ti) -> (* TODO: remove cheating for IH *)
-  wp_app wp E nil t ===> wp_triple_ E t.
+Lemma wp_sound_redunop_int : forall (F:int->val) op v1,
+  (forall (n1:int), redunop op n1 (F n1)) ->
+  wp_unop_int v1 F ===> wp_triple (trm_apps op (trms_vals (v1::nil))).
 Proof using.
-  introv IHwp. cuts M: (forall vs,  
-   wp_app wp E vs t ===> wp_triple_ E (trm_apps t (trms_vals vs))).
-  { applys M. }
-  induction t; intros; try solve [  simpl; apply qimpl_wp_fail_l ].
-  applys wp_sound_getval (fun t2 => 
-    trm_apps (trm_app t1 t2) (trms_vals vs)). 
-  { skip. (* TODO: rec eval ctx *) }
-  { applys IHwp. (* TODO: fix IH *) }
-  fold (wp_app wp E).
-  intros v2.
-  asserts Common: (wp_getval wp E t1 (fun v1 =>
-    wp_app_val E  (trm_apps v1 (trms_vals (v2::vs))))
-    ===> wp_triple_ E (trm_apps (t1 v2) (trms_vals vs))).
-  { applys wp_sound_getval (fun t1 => 
-    trm_apps (trm_app t1 v2) (trms_vals vs)). 
-    { skip. (* TODO: rec eval ctx *) } 
-    { apply IHwp. (* TODO: fix IH *) }
-    { intros v1. applys wp_sound_app_val. } }
-  destruct t1; try apply Common.
-  { lets IH: IHt1 (v2::vs). apply IH. }
+  introv M. applys qimpl_wp_triple; intros Q; simpl.
+  remove_local. intros n1 ->. applys triple_combined.
+  { applys triple_unop M. } { hsimpl. } { hpull ;=> ? ->. hsimpl. }
+Qed.
+
+Lemma wp_sound_redunop_bool : forall (F:bool->val) op v1,
+  (forall (b1:bool), redunop op b1 (F b1)) ->
+  wp_unop_bool v1 F ===> wp_triple (trm_apps op (trms_vals (v1::nil))).
+Proof using.
+  introv M. applys qimpl_wp_triple; intros Q; simpl.
+  remove_local. intros n1 ->. applys triple_combined.
+  { applys triple_unop M. } { hsimpl. } { hpull ;=> ? ->. hsimpl. }
+Qed.
+
+Lemma wp_sound_redbinop_int : forall (F:int->int->val) op v1 v2,
+  (forall (n1 n2:int), redbinop op n1 n2 (F n1 n2)) ->
+  wp_binop_int v1 v2 F ===> wp_triple (trm_apps op (trms_vals (v1::v2::nil))).
+Proof using.
+  introv M. applys qimpl_wp_triple; intros Q; simpl.
+  remove_local. intros n1 n2 (->&->). applys triple_combined.
+  { applys triple_binop M. } { hsimpl. } { hpull ;=> ? ->. hsimpl. }
+Qed.
+
+Lemma wp_sound_apps_val : forall v0 vs,
+  wp_apps_val v0 vs ===> wp_triple (trm_apps v0 vs). (* no subst *)
+Proof using.
+  Hint Constructors redunop redbinop.
+  intros.
+  asserts Common: (local (wp_triple (trm_apps v0 vs)) ===> wp_triple (trm_apps v0 vs)).
+  { apply~ local_erase_l. { applys is_local_wp_triple. } }
+  intros Q. destruct v0; try solve [ apply Common ].
+  rename p into p. destruct p; try solve [ apply Common ];
+   destruct vs as [|v1 [|v2 [|]]]; try solve [ apply Common ].
+  { applys* wp_sound_redunop_bool. }
+  { applys* wp_sound_redunop_int. }
+  { applys* wp_sound_redbinop. }
+  { applys* wp_sound_redbinop. eauto. }
+  { applys* wp_sound_redbinop_int. }
+  { applys* wp_sound_redbinop_int. }
+  { applys* wp_sound_redbinop_int. }
+Qed.
+
+Lemma wp_sound_apps : forall t0 ts,
+  wp_sound t0 ->
+  (forall t, mem t ts -> wp_sound t) ->
+  wp_sound (trm_apps t0 ts).
+Proof using.
+  introv IH0 IHts. intros E Q. applys~ wp_sound_getval (fun t1 => trm_apps t1 ts).
+  fold wp. intros v0. clear Q.
+  cuts M: (forall rvs,  
+    wp_apps wp E v0 rvs ts ===> 
+    wp_triple (trm_apps v0 ((trms_vals (LibList.rev rvs))++(LibList.map (isubst E) ts)))).
+  { unfold wp_triple_. simpl. rewrite List_map_eq. applys M. }
+  induction ts as [|t ts']; intros.
+  { simpl. rewrite List_rev_eq. rew_list. applys wp_sound_apps_val. }
+  { specializes IHts' __. { intros t' Ht'. applys* IHts. }
+    unfold wp_apps. fold (wp_apps wp E v0). rew_listx.
+    forwards~ M: wp_sound_getval E (fun t1 => trm_apps v0 (trms_vals (rev rvs) ++ t1 :: ts')).
+    2:{ unfold wp_triple_ in M. rewrite isubst_trm_apps_app in M. applys M. }
+    intros v1. applys qimpl_wp_triple. intros Q.
+    rewrite isubst_trm_apps_args. simpl. apply triple_of_wp.
+    forwards M: IHts' (v1::rvs). rewrite app_trms_vals_rev_cons in M. applys M. }
 Qed.
 
 Lemma wp_sound_while : forall F1 F2 E t1 t2,
@@ -584,13 +642,13 @@ Proof using.
   { split.
     { applys is_local_wp_triple. }
     { clears Q. applys qimpl_wp_triple. intros Q.
-      applys triple_while_raw. rewrite~ triple_eq_himpl_wp_triple.
+      applys triple_while_raw. apply~ triple_of_wp.
       change ((trm_if (isubst E t1) (trm_seq (isubst E t2) (trm_while (isubst E t1) (isubst E t2))) val_unit))
         with (isubst E (trm_if t1 (trm_seq t2 (trm_while t1 t2)) val_unit)).
       applys~ wp_sound_if. 
       { applys* wp_sound_seq. eauto. }
       { intros Q'. applys wp_sound_val. } } }
-  { rewrite~ triple_eq_himpl_wp_triple. }
+  { apply~ triple_of_wp. }
 Qed.
 
 Lemma wp_sound_for_val : forall (x:var) v1 v2 F1 E t1,
@@ -606,7 +664,7 @@ Proof using. Opaque Ctx.add Ctx.rem.
     { intros r. applys is_local_wp_triple. }
     { clears Q. intros i. applys qimpl_wp_triple. intros Q.
       applys triple_for_raw. fold isubst.
-      rewrite~ triple_eq_himpl_wp_triple. case_if.
+      apply~ triple_of_wp. case_if.
       { rewrite <- isubst_add_eq_subst1_isubst.
         asserts_rewrite (trm_seq (isubst (Ctx.add x (val_int i) E) t1) (trm_for x (i + 1)%I n2 (isubst (Ctx.rem x E) t1))
           = (isubst (Ctx.add x (val_int i) E) (trm_seq t1 (trm_for x (i + 1)%I n2 t1)))).
@@ -615,16 +673,16 @@ Proof using. Opaque Ctx.add Ctx.rem.
         { applys* M. }
         { unfold S. unfold wp_triple_. simpl. rewrite~ Ctx.rem_add_same. } }
       { applys wp_sound_val E. } } }
-  { rewrite~ triple_eq_himpl_wp_triple. }
+  { apply~ triple_of_wp. }
 Qed.
 
-Lemma wp_sound_for_trm : forall x t1 t2 t3 E,
+Lemma wp_sound_for_trm : forall x t1 t2 t3,
   wp_sound t1 ->
   wp_sound t2 ->
   wp_sound t3 ->
-  wp E (trm_for x t1 t2 t3) ===> wp_triple_ E (trm_for x t1 t2 t3).
+  wp_sound (trm_for x t1 t2 t3).
 Proof using.
-  introv M1 M2 M3. intros Q. simpl.
+  introv M1 M2 M3. intros E Q. simpl.
   applys~ wp_sound_getval (fun t1 => trm_for x t1 t2 t3).
   intros v1. applys~ wp_sound_getval (fun t2 => trm_for x v1 t2 t3).
   intros v2. applys~ wp_sound_for_val.
@@ -639,19 +697,19 @@ Proof using.
   remove_local. applys triple_case.
   { intros G HG Hv1. rewrites <- (rm HG).
     applys triple_hand_l. applys triple_hforall_for G.
-    applys~ triple_hwand_hpure_l. rewrite triple_eq_himpl_wp_triple.
+    applys~ triple_hwand_hpure_l. apply triple_of_wp.
     rewrite <- isubst_app_eq_isubst_isubst_rem_vars. applys M1. }
   { introv Hv1. applys triple_hand_r. applys* triple_hwand_hpure_l. 
-    rewrite triple_eq_himpl_wp_triple. applys M2. }
+    apply triple_of_wp. applys M2. }
 Qed.
 
-Lemma wp_sound_case_trm : forall t1 p t2 t3 E,
+Lemma wp_sound_case_trm : forall t1 p t2 t3,
   wp_sound t1 ->
   wp_sound t2 ->
   wp_sound t3 ->
-  wp E (trm_case t1 p t2 t3) ===> wp_triple_ E (trm_case t1 p t2 t3).
+  wp_sound (trm_case t1 p t2 t3).
 Proof using.
-  introv M1 M2 M3. intros Q. simpl.
+  introv M1 M2 M3. intros E Q. simpl.
   applys~ wp_sound_getval (fun t1 => trm_case t1 p t2 t3).
   intros v. applys~ wp_sound_case_val.
 Qed.
@@ -671,8 +729,8 @@ Proof using.
     applys~ wp_sound_getval (fun t1 => trm_constr id (trms_vals (rev rvs) ++ t1 :: ts')).
     intros v1. fold (wp_constr wp E id).
     applys qimpl_wp_triple. intros Q. rewrite isubst_trm_constr_args.
-    rewrite triple_eq_himpl_wp_triple.
-    forwards M: IHts' (v1::rvs). rew_listx~ in M.
+    apply triple_of_wp.
+    forwards M: IHts' (v1::rvs). unfold trms_vals in *. rew_listx~ in M.
     unfold wp_triple_ in M. rewrite isubst_trm_constr_args in M. apply M. }
 Qed.
 
@@ -682,11 +740,11 @@ Proof using.
   intros t. induction t using trm_induct; intros E Q.
   { applys wp_sound_val. }
   { applys wp_sound_var. }
-  { applys wp_sound_fix. }
+  { applys wp_sound_fixs. }
   { applys* wp_sound_constr Q. }
   { applys* wp_sound_if. }
   { applys* wp_sound_let. }
-  { applys* wp_sound_app. skip. (* TODO IH *) }
+  { applys* wp_sound_apps. }
   { applys* wp_sound_while. }
   { applys* wp_sound_for_trm. }
   { applys* wp_sound_case_trm. }
@@ -700,7 +758,7 @@ Qed.
 Lemma triple_isubst_wp : forall t E Q,
   triple (isubst E t) (wp E t Q) Q.
 Proof using.
-  intros. rewrite triple_eq_himpl_wp_triple. applys wp_sound_trm.
+  intros. apply triple_of_wp. applys wp_sound_trm.
 Qed.
 
 Lemma triple_isubst_of_wp : forall t E H Q,
@@ -708,7 +766,7 @@ Lemma triple_isubst_of_wp : forall t E H Q,
   triple (isubst E t) H Q.
 Proof using. introv M. xchanges M. applys triple_isubst_wp. Qed.
 
-Lemma triple_of_wp : forall (t:trm) H Q,
+Lemma triple_of_wp_empty : forall (t:trm) H Q,
   H ==> wp Ctx.empty t Q ->
   triple t H Q.
 Proof using.
@@ -744,22 +802,17 @@ Lemma is_local_wp : forall E t,
 Proof.
   intros. induction t using trm_induct; try solve [ simpl; eauto ]. 
   { simpl. rename v into x. simpl. unfold wp_var. destruct_lookup~. }
+  { simpl. destruct~ xs. }
   { simpl. rename l into ts. simpl. generalize (@nil val) as rvs.
-    induction ts as [|t ts']; intros; auto.
+    induction ts as [|t' ts']; intros; auto.
     { applys* is_local_wp_getval. } }
-  { (* TODO: fix induction: and state as separate lemma?, like is_local_constr *)
-    unfold wp; fold wp. 
-    generalize (@nil val) as vs. 
-    generalize (trm_app t1 t2) as t. clears t1 t2.
-    induction t; intros; auto. 
-    { simpl. applys* is_local_wp_getval.
-      { skip. (* IH *) }
-      { intros v2. destruct t1; 
-         try solve [ apply is_local_local | applys is_local_wp_getval ]. (* auto *)
-        { applys is_local_wp_getval. 
-          { skip. (* IH *) }
-          { intros v1. auto. } }
-        { applys IHt1. } (* auto. *) } } }
+  { simpl. applys* is_local_wp_getval. intros v0.
+    rename l into ts. simpl. generalize (@nil val) as rvs.
+    induction ts as [|t' ts']; intros; auto.
+    { simpl. generalize (List.rev rvs) as vs. intros.
+      unfolds wp_apps. destruct~ v0.
+      destruct~ p; destruct vs as [|v1 [|v2 [ | ]]]; auto. }
+    { applys* is_local_wp_getval. } }
 Qed.
 
 End IsLocalWp.
